WIP

ems/SimGlobalAlts.v
@@ -11,7 +11,37 @@ Require Import RelationPairs.
 From Ordinal Require Import Ordinal Arithmetic.
 From Ordinal Require Import ClassicalOrdinal.
 
+Require Import WFLib.
+
 Set Implicit Arguments.
+
+Section COMMON.
+
+  Variable R: Type.
+  Let ITR := (itree eventE R).
+
+  Variant obs_step (args: string * Any.t * (Any.t -> Prop) * Any.t) (r: ITR -> Prop): ITR -> Prop :=
+    | obs_step_syscall
+        fn varg rvs ktr v
+        (REL: r (ktr v))
+        (ARGS: args = (fn, varg, rvs, v))
+      :
+      obs_step args r (trigger (Syscall fn varg rvs) >>= ktr)
+  .
+
+  Variant is_ret (rv: R): ITR -> Prop :=
+    | is_ret_intro: is_ret rv (Ret rv).
+
+  Lemma obs_step_mon
+        args (r0 r1: ITR -> Prop) itr
+        (MON: forall itr, (r0 itr) -> (r1 itr))
+    :
+    (obs_step args r0 itr) -> (obs_step args r1 itr).
+  Proof.
+    i. inv H. econs; eauto.
+  Qed.
+
+End COMMON.
 
 Section SRCSTEPS.
 
@@ -38,386 +68,169 @@ Section SRCSTEPS.
   .
 
   Inductive st_star (r: ITR -> Prop): ITR -> Prop :=
-  | base itr (REL: r itr): st_star r itr
-  | step itr (REL: st_step (fun ktr => st_star r ktr) itr): st_star r itr
-  .
-
-  Variant so_step (args: string * Any.t * (Any.t -> Prop) * Any.t) (r: ITR -> Prop): ITR -> Prop :=
-    | so_step_syscall
-        fn varg rvs ktr v
-        (REL: r (ktr v))
-        (ARGS: args = (fn, varg, rvs, v))
-      :
-      so_step args r (trigger (Syscall fn varg rvs) >>= ktr)
+  | st_star_base itr (REL: r itr): st_star r itr
+  | st_star_step itr (REL: st_step (fun ktr => st_star r ktr) itr): st_star r itr
   .
 
   Definition src_step (r: (option (string * Any.t * (Any.t -> Prop) * Any.t)) -> ITR -> Prop):
     ITR -> Prop :=
     fun itr =>
-      (<<TAU: st_step (r None) itr>>) \/ (<<OBS: exists args, so_step args (r (Some args)) itr>>)
+      (<<TAU: st_step (r None) itr>>) \/ (<<OBS: exists args, obs_step args (r (Some args)) itr>>)
   .
 
   Definition src_plus (r: (option (string * Any.t * (Any.t -> Prop) * Any.t)) -> ITR -> Prop):
-    ITR -> Prop :=
-    fun itr => (st_star (fun ktr => src_step r ktr) itr)
+    ITR -> Prop := (st_star (fun ktr => src_step r ktr))
   .
 
-  Variant is_return: ITR -> Prop :=
-    | is_return_intro retv: is_return (Ret retv).
+  (* properties *)
+  Lemma st_step_mon
+        (r0 r1: ITR -> Prop) itr
+        (MON: forall itr, (r0 itr) -> (r1 itr))
+    :
+    (st_step r0 itr) -> (st_step r1 itr).
+  Proof.
+    i. inv H; econs; eauto. des. eauto.
+  Qed.
+
+  Lemma st_star_ind2 (r: ITR -> Prop) (P: ITR -> Prop)
+        (BASE: forall itr (REL: r itr), P itr)
+        (STEP: forall itr (REL: st_step (fun ktr => (<<STAR: st_star r ktr>>) /\ (<<IH: P ktr>>)) itr),
+            P itr)
+    :
+    forall itr (STAR: st_star r itr), P itr.
+  Proof.
+    fix IH 2. i. inv STAR. eauto.
+    eapply STEP. inv REL.
+    { econs 1. split; auto. }
+    { econs 2. des. exists x. split; auto. }
+    { econs 3. i. split; auto. }
+  Qed.
+
+  Lemma st_star_mon
+        (r0 r1: ITR -> Prop) itr
+        (MON: forall itr, (r0 itr) -> (r1 itr))
+    :
+    (st_star r0 itr) -> (st_star r1 itr).
+  Proof.
+    i. induction H using st_star_ind2. econs 1; eauto.
+    econs 2. eapply st_step_mon. 2: eauto. i; ss. des. auto.
+  Qed.
+
+  Lemma src_step_mon
+        (r0 r1: (option (string * Any.t * (Any.t -> Prop) * Any.t)) -> ITR -> Prop) itr
+        (MON: forall args itr, (r0 args itr) -> (r1 args itr))
+    :
+    (src_step r0 itr) -> (src_step r1 itr).
+  Proof.
+    i. inv H.
+    - econs 1. eapply st_step_mon. 2: eauto. eauto.
+    - des. econs 2. exists args. eapply obs_step_mon. 2: eauto. eauto.
+  Qed.
+
+  Lemma src_plus_mon
+        (r0 r1: (option (string * Any.t * (Any.t -> Prop) * Any.t)) -> ITR -> Prop) itr
+        (MON: forall args itr, (r0 args itr) -> (r1 args itr))
+    :
+    (src_plus r0 itr) -> (src_plus r1 itr).
+  Proof.
+    i. eapply st_star_mon. 2: eauto. i; ss. eapply src_step_mon. 2: eauto. eauto.
+  Qed.
 
 End SRCSTEPS.
 
+Section TGTSTEPS.
+
+  Variable R: Type.
+  Let ITR := (itree eventE R).
+
+  (* tgt tau step *)
+  Variant tt_step (r: ITR -> Prop): ITR -> Prop :=
+    | tt_step_tau
+        ktr
+        (REL: r ktr)
+      :
+      tt_step r (tau;; ktr)
+    | tt_step_choose
+        X ktr
+        (REL: forall x, r (ktr x))
+      :
+      tt_step r (trigger (Choose X) >>= ktr)
+    | tt_step_take
+        X ktr
+        (REL: exists x, r (ktr x))
+      :
+      tt_step r (trigger (Take X) >>= ktr)
+  .
+
+  Definition tgt_step (r: (option (string * Any.t * (Any.t -> Prop) * Any.t)) -> ITR -> Prop):
+    ITR -> Prop :=
+    fun itr =>
+      (<<TAU: tt_step (r None) itr>>) \/ (<<OBS: exists args, obs_step args (r (Some args)) itr>>)
+  .
+
+  (* properties *)
+  Lemma tt_step_mon
+        (r0 r1: ITR -> Prop) itr
+        (MON: forall itr, (r0 itr) -> (r1 itr))
+    :
+    (tt_step r0 itr) -> (tt_step r1 itr).
+  Proof.
+    i. inv H; econs; eauto. des. eauto.
+  Qed.
+
+  Lemma tgt_step_mon
+        (r0 r1: (option (string * Any.t * (Any.t -> Prop) * Any.t)) -> ITR -> Prop) itr
+        (MON: forall args itr, (r0 args itr) -> (r1 args itr))
+    :
+    (tgt_step r0 itr) -> (tgt_step r1 itr).
+  Proof.
+    i. inv H.
+    - econs 1. eapply tt_step_mon. 2: eauto. eauto.
+    - des. econs 2. exists args. eapply obs_step_mon. 2: eauto. eauto.
+  Qed.
+
+End TGTSTEPS.
 
 
-Section SIM.
 
-Inductive _simg
-          (simg: forall R0 R1 (RR: Ord.t -> Ord.t -> R0 -> R1 -> Prop), Ord.t -> Ord.t -> (itree eventE R0) -> (itree eventE R1) -> Prop)
-          {R0 R1} (RR: Ord.t -> Ord.t -> R0 -> R1 -> Prop) (f_src f_tgt: Ord.t): (itree eventE R0) -> (itree eventE R1) -> Prop :=
-| simg_ret
-    r_src r_tgt
-    (SIM: RR f_src f_tgt r_src r_tgt)
-  :
-    _simg simg RR f_src f_tgt (Ret r_src) (Ret r_tgt)
-| simg_syscall
-    ktr_src0 ktr_tgt0 fn varg rvs
-    f_src0 f_tgt0
-    (SIM: forall x_src x_tgt (EQ: x_src = x_tgt), simg _ _ RR f_src0 f_tgt0 (ktr_src0 x_src) (ktr_tgt0 x_tgt))
-  :
-    _simg simg RR f_src f_tgt (trigger (Syscall fn varg rvs) >>= ktr_src0) (trigger (Syscall fn varg rvs) >>= ktr_tgt0)
+Section EXP_SIM.
 
-| simg_tauL
-    itr_src0 itr_tgt0
-    (TAUL: True)
-    f_src0
-    (SIM: @_simg simg _ _ RR f_src0 f_tgt itr_src0 itr_tgt0)
-  :
-    _simg simg RR f_src f_tgt (tau;; itr_src0) (itr_tgt0)
-| simg_tauR
-    itr_src0 itr_tgt0
-    (TAUR: True)
-    f_tgt0
-    (SIM: @_simg simg _ _ RR f_src f_tgt0 itr_src0 itr_tgt0)
-  :
-    _simg simg RR f_src f_tgt (itr_src0) (tau;; itr_tgt0)
+  Variable wfo: WF.
 
-| simg_chooseL
-    X ktr_src0 itr_tgt0
-    (CHOOSEL: True)
-    f_src0
-    (SIM: exists x, _simg simg RR f_src0 f_tgt (ktr_src0 x) itr_tgt0)
-  :
-    _simg simg RR f_src f_tgt (trigger (Choose X) >>= ktr_src0) (itr_tgt0)
-| simg_chooseR
-    X itr_src0 ktr_tgt0
-    (CHOOSER: True)
-    f_tgt0
-    (SIM: forall x, _simg simg RR f_src f_tgt0 itr_src0 (ktr_tgt0 x))
-  :
-    _simg simg RR f_src f_tgt (itr_src0) (trigger (Choose X) >>= ktr_tgt0)
+  Definition _simg_alt_exp
+             (simg_alt_exp: forall R0 R1 (RR: R0 -> R1 -> Prop), wfo.(T) -> (itree eventE R0) -> (itree eventE R1) -> Prop)
+             {R0 R1} (RR: R0 -> R1 -> Prop) (f_tgt: wfo.(T)): (itree eventE R0) -> (itree eventE R1) -> Prop :=
+    fun itr_src itr_tgt =>
+      (<<RET: exists rt, (<<RETTGT: is_ret rt itr_tgt>>) ->
+                    (<<RETSRC: st_star (fun ktr => exists rs, (is_ret rs ktr) /\ (RR rs rt)) itr_src>>)>>)
+      /\
+        (
+          (<<STAR: (tt_step (fun ktr_tgt => (st_star (fun ktr_src => exists f_tgt0, (simg_alt_exp _ _ RR f_tgt0 ktr_src ktr_tgt) /\ (wfo.(lt) f_tgt0 f_tgt)) itr_src)) itr_tgt)>>)
+          \/
+            (<<PLUS: (tgt_step (fun targs ktr_tgt => (src_plus (fun sargs ktr_src => exists f_tgt0, (simg_alt_exp _ _ RR f_tgt0 ktr_src ktr_tgt) /\ (targs = sargs)) itr_src)) itr_tgt)>>)
+        )
+  .
 
-| simg_takeL
-    X ktr_src0 itr_tgt0
-    (TAKEL: True)
-    f_src0
-    (SIM: forall x, _simg simg RR f_src0 f_tgt (ktr_src0 x) itr_tgt0)
-  :
-    _simg simg RR f_src f_tgt (trigger (Take X) >>= ktr_src0) (itr_tgt0)
-| simg_takeR
-    X itr_src0 ktr_tgt0
-    (TAKER: True)
-    f_tgt0
-    (SIM: exists x, _simg simg RR f_src f_tgt0 itr_src0 (ktr_tgt0 x))
-  :
-    _simg simg RR f_src f_tgt (itr_src0) (trigger (Take X) >>= ktr_tgt0)
+  Definition simg_alt_exp: forall R0 R1 (RR: R0 -> R1 -> Prop), wfo.(T) -> (itree eventE R0) -> (itree eventE R1) -> Prop := paco6 _simg_alt_exp bot6.
 
-| simg_progress
-    itr_src itr_tgt
-    f_src0 f_tgt0
-    (SIM: simg _ _ RR f_src0 f_tgt0 itr_src itr_tgt)
-    (SRC: (f_src0 < f_src)%ord)
-    (TGT: (f_tgt0 < f_tgt)%ord)
-  :
-    _simg simg RR f_src f_tgt itr_src itr_tgt
-.
+  Lemma simg_alt_exp_mon: monotone6 _simg_alt_exp.
+  Proof.
+    ii. inv IN. des.
+    { unfold _simg_alt_exp. split; eauto.
+      left. eapply tt_step_mon. 2: eauto. i; ss. eapply st_star_mon. 2: eauto. i; ss.
+      des. eauto.
+    }
+    { unfold _simg_alt_exp. split; eauto.
+      right. eapply tgt_step_mon. 2: eauto. i; ss. eapply src_plus_mon. 2: eauto. i; ss.
+      des. eauto.
+    }
+  Qed.
 
-Lemma _simg_ind2 (r: forall R0 R1 (RR: Ord.t -> Ord.t -> R0 -> R1 -> Prop), Ord.t -> Ord.t -> (itree eventE R0) -> (itree eventE R1) -> Prop)
-      R0 R1 (RR: Ord.t -> Ord.t -> R0 -> R1 -> Prop)
-      (P: Ord.t -> Ord.t -> (itree eventE R0) -> (itree eventE R1) -> Prop)
-      (RET: forall
-          f_src f_tgt
-          r_src r_tgt
-          (SIM: RR f_src f_tgt r_src r_tgt),
-          P f_src f_tgt (Ret r_src) (Ret r_tgt))
-      (SYSCALL: forall
-          f_src f_tgt
-          f_src0 f_tgt0
-          ktr_src0 ktr_tgt0 fn varg rvs
-          (SIM: forall x_src x_tgt (EQ: x_src = x_tgt), r _ _ RR f_src0 f_tgt0 (ktr_src0 x_src) (ktr_tgt0 x_tgt)),
-          P f_src f_tgt (trigger (Syscall fn varg rvs) >>= ktr_src0) (trigger (Syscall fn varg rvs) >>= ktr_tgt0))
-      (TAUL: forall
-          f_src0
-          f_src f_tgt
-          itr_src0 itr_tgt0
-          (TAUL: True)
-          (SIM: _simg r RR f_src0 f_tgt itr_src0 itr_tgt0)
-          (IH: P f_src0 f_tgt itr_src0 itr_tgt0),
-          P f_src f_tgt (tau;; itr_src0) (itr_tgt0))
-      (TAUR: forall
-          f_tgt0
-          f_src f_tgt
-          itr_src0 itr_tgt0
-          (TAUR: True)
-          (SIM: _simg r RR f_src f_tgt0 itr_src0 itr_tgt0)
-          (IH: P f_src f_tgt0 itr_src0 itr_tgt0),
-          P f_src f_tgt (itr_src0) (tau;;itr_tgt0))
-      (CHOOSEL: forall
-          f_src0
-          f_src f_tgt
-          X ktr_src0 itr_tgt0
-          (CHOOSEL: True)
-          (SIM: exists x, <<SIM: _simg r RR f_src0 f_tgt (ktr_src0 x) itr_tgt0>> /\ <<IH: P f_src0 f_tgt (ktr_src0 x) itr_tgt0>>),
-          P f_src f_tgt (trigger (Choose X) >>= ktr_src0) (itr_tgt0))
-      (CHOOSER: forall
-          f_tgt0
-          f_src f_tgt
-          X itr_src0 ktr_tgt0
-          (CHOOSER: True)
-          (SIM: forall x, <<SIM: _simg r RR f_src f_tgt0 itr_src0 (ktr_tgt0 x)>> /\ <<IH: P f_src f_tgt0 itr_src0 (ktr_tgt0 x)>>),
-          P f_src f_tgt (itr_src0) (trigger (Choose X) >>= ktr_tgt0))
-      (TAKEL: forall
-          f_src0
-          f_src f_tgt
-          X ktr_src0 itr_tgt0
-          (TAKEL: True)
-          (SIM: forall x, <<SIM: _simg r RR f_src0 f_tgt (ktr_src0 x) itr_tgt0>> /\ <<IH: P f_src0 f_tgt (ktr_src0 x) itr_tgt0>>),
-          P f_src f_tgt (trigger (Take X) >>= ktr_src0) (itr_tgt0))
-      (TAKER: forall
-          f_tgt0
-          f_src f_tgt
-          X itr_src0 ktr_tgt0
-          (TAKER: True)
-          (SIM: exists x, <<SIM: _simg r RR f_src f_tgt0 itr_src0 (ktr_tgt0 x)>> /\ <<IH: P f_src f_tgt0 itr_src0 (ktr_tgt0 x)>>),
-          P f_src f_tgt (itr_src0) (trigger (Take X) >>= ktr_tgt0))
-      (PROGRESS: forall
-          f_src0 f_tgt0
-          f_src f_tgt
-          itr_src itr_tgt
-          (SIM: r _ _ RR f_src0 f_tgt0 itr_src itr_tgt)
-          (SRC: (f_src0 < f_src)%ord)
-          (TGT: (f_tgt0 < f_tgt)%ord),
-          P f_src f_tgt itr_src itr_tgt)
-  :
-    forall f_src f_tgt itr_src itr_tgt
-           (SIM: _simg r RR f_src f_tgt itr_src itr_tgt),
-      P f_src f_tgt itr_src itr_tgt.
-Proof.
-  fix IH 5. i. inv SIM.
-  { eapply RET; eauto. }
-  { eapply SYSCALL; eauto. }
-  { eapply TAUL; eauto. }
-  { eapply TAUR; eauto. }
-  { eapply CHOOSEL; eauto. des. esplits; eauto. }
-  { eapply CHOOSER; eauto. }
-  { eapply TAKEL; eauto. }
-  { eapply TAKER; eauto. des. esplits; eauto. }
-  { eapply PROGRESS; eauto. }
-Qed.
-
-Definition simg: forall R0 R1 (RR: Ord.t -> Ord.t -> R0 -> R1 -> Prop), Ord.t -> Ord.t -> (itree eventE R0) -> (itree eventE R1) -> Prop := paco7 _simg bot7.
-
-Lemma simg_mon: monotone7 _simg.
-Proof.
-  ii. induction IN using _simg_ind2.
-  { econs 1; eauto. }
-  { econs 2; eauto. }
-  { econs 3; eauto. }
-  { econs 4; eauto. }
-  { econs 5; eauto. des. esplits; eauto. }
-  { econs 6; eauto. i. spc SIM. des; et. }
-  { econs 7; eauto. i. spc SIM. des; et. }
-  { econs 8; eauto. des. esplits; eauto. }
-  { econs 9; eauto. }
-Qed.
-Hint Resolve simg_mon: paco.
-Hint Resolve cpn7_wcompat: paco.
+  Hint Resolve simg_alt_exp_mon: paco.
+  Hint Resolve cpn6_wcompat: paco.
 
 
-Variant simg_indC
-          (simg: forall R0 R1 (RR: Ord.t -> Ord.t -> R0 -> R1 -> Prop), Ord.t -> Ord.t -> (itree eventE R0) -> (itree eventE R1) -> Prop)
-          {R0 R1} (RR: Ord.t -> Ord.t -> R0 -> R1 -> Prop) (f_src f_tgt: Ord.t): (itree eventE R0) -> (itree eventE R1) -> Prop :=
-| simg_indC_ret
-    r_src r_tgt
-    (SIM: RR f_src f_tgt r_src r_tgt)
-  :
-    simg_indC simg RR f_src f_tgt (Ret r_src) (Ret r_tgt)
-| simg_indC_syscall
-    f_src0 f_tgt0
-    ktr_src0 ktr_tgt0 fn varg rvs
-    (SIM: forall x_src x_tgt (EQ: x_src = x_tgt), simg _ _ RR f_src0 f_tgt0 (ktr_src0 x_src) (ktr_tgt0 x_tgt))
-  :
-    simg_indC simg RR f_src f_tgt (trigger (Syscall fn varg rvs) >>= ktr_src0) (trigger (Syscall fn varg rvs) >>= ktr_tgt0)
-
-| simg_indC_tauL
-    f_src0
-    itr_src0 itr_tgt0
-    (TAUL: True)
-    (SIM: simg _ _ RR f_src0 f_tgt itr_src0 itr_tgt0)
-  :
-    simg_indC simg RR f_src f_tgt (tau;; itr_src0) (itr_tgt0)
-| simg_indC_tauR
-    f_tgt0
-    itr_src0 itr_tgt0
-    (TAUR: True)
-    (SIM: simg _ _ RR f_src f_tgt0 itr_src0 itr_tgt0)
-  :
-    simg_indC simg RR f_src f_tgt (itr_src0) (tau;; itr_tgt0)
-
-| simg_indC_chooseL
-    f_src0
-    X ktr_src0 itr_tgt0
-    (CHOOSEL: True)
-    (SIM: exists x, simg _ _ RR f_src0 f_tgt (ktr_src0 x) itr_tgt0)
-  :
-    simg_indC simg RR f_src f_tgt (trigger (Choose X) >>= ktr_src0) (itr_tgt0)
-| simg_indC_chooseR
-    f_tgt0
-    X itr_src0 ktr_tgt0
-    (CHOOSER: True)
-    (SIM: forall x, simg _ _ RR f_src f_tgt0 itr_src0 (ktr_tgt0 x))
-  :
-    simg_indC simg RR f_src f_tgt (itr_src0) (trigger (Choose X) >>= ktr_tgt0)
-
-| simg_indC_takeL
-    f_src0
-    X ktr_src0 itr_tgt0
-    (TAKEL: True)
-    (SIM: forall x, simg _ _ RR f_src0 f_tgt (ktr_src0 x) itr_tgt0)
-  :
-    simg_indC simg RR f_src f_tgt (trigger (Take X) >>= ktr_src0) (itr_tgt0)
-| simg_indC_takeR
-    f_tgt0
-    X itr_src0 ktr_tgt0
-    (TAKER: True)
-    (SIM: exists x, simg _ _ RR f_src f_tgt0 itr_src0 (ktr_tgt0 x))
-  :
-    simg_indC simg RR f_src f_tgt (itr_src0) (trigger (Take X) >>= ktr_tgt0)
-.
-
-Lemma simg_indC_mon: monotone7 simg_indC.
-Proof.
-  ii. inv IN.
-  { econs 1; eauto. }
-  { econs 2; eauto. }
-  { econs 3; eauto. }
-  { econs 4; eauto. }
-  { econs 5; eauto. des. esplits; eauto. }
-  { econs 6; eauto. }
-  { econs 7; eauto. }
-  { econs 8; eauto. des. esplits; eauto. }
-Qed.
-Hint Resolve simg_indC_mon: paco.
-
-Lemma simg_indC_spec:
-  simg_indC <8= gupaco7 _simg (cpn7 _simg).
-Proof.
-  eapply wrespect7_uclo; eauto with paco.
-  econs; eauto with paco. i. inv PR.
-  { econs 1; eauto. }
-  { econs 2; eauto. i. eapply rclo7_base. auto. }
-  { econs 3; eauto. eapply simg_mon; eauto. i. eapply rclo7_base. auto. }
-  { econs 4; eauto. eapply simg_mon; eauto. i. eapply rclo7_base. auto. }
-  { des. econs 5; eauto. esplits. eapply simg_mon; eauto. i. eapply rclo7_base; eauto. }
-  { econs 6; eauto. i. eapply simg_mon; eauto. i. eapply rclo7_base; eauto. }
-  { econs 7; eauto. i. eapply simg_mon; eauto. i. eapply rclo7_base; eauto. }
-  { des. econs 8; eauto. esplits. eapply simg_mon; eauto. i. eapply rclo7_base; eauto. }
-Qed.
-
-Lemma simg_ind R0 R1 (RR: Ord.t -> Ord.t -> R0 -> R1 -> Prop)
-      (P: Ord.t -> Ord.t -> (itree eventE R0) -> (itree eventE R1) -> Prop)
-      (RET: forall
-          f_src f_tgt
-          r_src r_tgt
-          (SIM: RR f_src f_tgt r_src r_tgt),
-          P f_src f_tgt (Ret r_src) (Ret r_tgt))
-      (SYSCALL: forall
-          f_src0 f_tgt0
-          f_src f_tgt
-          ktr_src0 ktr_tgt0 fn varg rvs
-          (SIM: forall x_src x_tgt (EQ: x_src = x_tgt), simg RR f_src0 f_tgt0 (ktr_src0 x_src) (ktr_tgt0 x_tgt)),
-          P f_src f_tgt (trigger (Syscall fn varg rvs) >>= ktr_src0) (trigger (Syscall fn varg rvs) >>= ktr_tgt0))
-      (TAUL: forall
-          f_src0
-          f_src f_tgt
-          itr_src0 itr_tgt0
-          (TAUL: True)
-          (SIM: simg RR f_src0 f_tgt itr_src0 itr_tgt0)
-          (IH: P f_src0 f_tgt itr_src0 itr_tgt0),
-          P f_src f_tgt (tau;; itr_src0) (itr_tgt0))
-      (TAUR: forall
-          f_tgt0
-          f_src f_tgt
-          itr_src0 itr_tgt0
-          (TAUR: True)
-          (SIM: simg RR f_src f_tgt0 itr_src0 itr_tgt0)
-          (IH: P f_src f_tgt0 itr_src0 itr_tgt0),
-          P f_src f_tgt (itr_src0) (tau;;itr_tgt0))
-      (CHOOSEL: forall
-          f_src0
-          f_src f_tgt
-          X ktr_src0 itr_tgt0
-          (CHOOSEL: True)
-          (SIM: exists x, <<SIM: simg RR f_src0 f_tgt (ktr_src0 x) itr_tgt0>> /\ <<IH: P f_src0 f_tgt (ktr_src0 x) itr_tgt0>>),
-          P f_src f_tgt (trigger (Choose X) >>= ktr_src0) (itr_tgt0))
-      (CHOOSER: forall
-          f_tgt0
-          f_src f_tgt
-          X itr_src0 ktr_tgt0
-          (CHOOSER: True)
-          (SIM: forall x, <<SIM: simg RR f_src f_tgt0 itr_src0 (ktr_tgt0 x)>> /\ <<IH: P f_src f_tgt0 itr_src0 (ktr_tgt0 x)>>),
-          P f_src f_tgt (itr_src0) (trigger (Choose X) >>= ktr_tgt0))
-      (TAKEL: forall
-          f_src0
-          f_src f_tgt
-          X ktr_src0 itr_tgt0
-          (TAKEL: True)
-          (SIM: forall x, <<SIM: simg RR f_src0 f_tgt (ktr_src0 x) itr_tgt0>> /\ <<IH: P f_src0 f_tgt (ktr_src0 x) itr_tgt0>>),
-          P f_src f_tgt (trigger (Take X) >>= ktr_src0) (itr_tgt0))
-      (TAKER: forall
-          f_tgt0
-          f_src f_tgt
-          X itr_src0 ktr_tgt0
-          (TAKER: True)
-          (SIM: exists x, <<SIM: simg RR f_src f_tgt0 itr_src0 (ktr_tgt0 x)>> /\ <<IH: P f_src f_tgt0 itr_src0 (ktr_tgt0 x)>>),
-          P f_src f_tgt (itr_src0) (trigger (Take X) >>= ktr_tgt0))
-      (PROGRESS: forall
-          f_src0 f_tgt0
-          f_src f_tgt
-          itr_src itr_tgt
-          (SIM: simg RR f_src0 f_tgt0 itr_src itr_tgt)
-          (SRC: (f_src0 < f_src)%ord)
-          (TGT: (f_tgt0 < f_tgt)%ord),
-          P f_src f_tgt itr_src itr_tgt)
-  :
-    forall f_src f_tgt itr_src itr_tgt
-           (SIM: simg RR f_src f_tgt itr_src itr_tgt),
-      P f_src f_tgt itr_src itr_tgt.
-Proof.
-  i. punfold SIM. induction SIM using _simg_ind2; i; clarify.
-  { eapply RET; eauto. }
-  { eapply SYSCALL; eauto. i. hexploit SIM; eauto. i. des. pclearbot. eauto. }
-  { eapply TAUL; eauto. pfold. auto. }
-  { eapply TAUR; eauto. pfold. auto. }
-  { eapply CHOOSEL; eauto. des. esplits; eauto. pfold. auto. }
-  { eapply CHOOSER; eauto. i. hexploit SIM; eauto. i. des. esplits; eauto. pfold. et. }
-  { eapply TAKEL; eauto. i. hexploit SIM; eauto. i. des. esplits; eauto. pfold. auto. }
-  { eapply TAKER; eauto. des. esplits; eauto. pfold. auto. }
-  { eapply PROGRESS; eauto. pclearbot. auto. }
-Qed.
-
-End SIM.
-
-Hint Constructors _simg.
-Hint Unfold simg.
-Hint Resolve simg_mon: paco.
-Hint Resolve cpn7_wcompat: paco.
+End EXP_SIM.
+Hint Unfold simg_alt_exp.
+Hint Resolve simg_alt_exp_mon: paco.
+Hint Resolve cpn6_wcompat: paco.
